separate Transpile_Tests

SepLogicTime/Transpile_Tests.thy
@@ -2,10 +2,7 @@ theory Transpile_Tests
   imports
   "SeprefTime.EdmondsKarp_Time"
   Transpile BinarySearch_Impl
- RBTree_Impl Skew_Heap_Impl DynamicArray2
-      "SeprefTime.Remdups" "SeprefTime.Kruskal_Time"
-  
- "SeprefTime.FW_Code"
+ RBTree_Impl Skew_Heap_Impl DynamicArray2 
   MergeSort_Impl
 
    "HOL-Library.Code_Target_Numeral"
@@ -17,43 +14,36 @@ schematic_goal p: "refines ?G (binarysearch l r x a)"
   apply(subst binarysearch.simps)
   apply(rule transpile_rules refines_flatten)+ done
 
-partial_function (heap) aahh where
-"aahh l r x a = (if r \<le> l then Heap_Monad.return False
+partial_function (heap) binarysearch_flat where
+"binarysearch_flat l r x a = (if r \<le> l then Heap_Monad.return False
   else if r \<le> l + 1 then Array.nth a l \<bind> (\<lambda>v. Heap_Monad.return (v = x))
        else let b = avg l r
             in Array.nth a b \<bind>
                (\<lambda>c. if c = x then Heap_Monad.return True
-                    else if c < x then aahh (b + 1) r x a else aahh l b x a))"
+                    else if c < x then binarysearch_flat (b + 1) r x a 
+                              else binarysearch_flat l b x a))"
 
-lemma refines_binarysearch: "refines (aahh l r x a) (binarysearch l r x a)"
+lemma refines_binarysearch: "refines (binarysearch_flat l r x a) (binarysearch l r x a)"
   unfolding refines_def
 proof safe
   fix h h' ra n
   assume *: "Heap_Time_Monad.effect (binarysearch l r x a) h h' ra n"
   
-  note f =  binarysearch.raw_induct[where P="\<lambda>l r x a h h' ra n. Heap_Monad.effect (aahh l r x a) h h' ra", where xa="(((l,r),x),a)", simplified]
+  note f =  binarysearch.raw_induct[where P="\<lambda>l r x a h h' ra n. Heap_Monad.effect (binarysearch_flat l r x a) h h' ra", where xa="(((l,r),x),a)", simplified]
 
-  show "Heap_Monad.effect (aahh l r x a) h h' ra" 
+  show "Heap_Monad.effect (binarysearch_flat l r x a) h h' ra" 
   proof (rule f[OF _ *], goal_cases) 
     case (1 f l r x a la ra xa aa)
-    from 1(1) have IH: "\<And>l r x a. refines (aahh l r x a) (f l r x a) " unfolding refines_def by auto 
+    from 1(1) have IH: "\<And>l r x a. refines (binarysearch_flat l r x a) (f l r x a) " unfolding refines_def by auto 
     show ?case apply(rule refinesD1[OF _ 1(2)])
-      apply(subst aahh.simps)
+      apply(subst binarysearch_flat.simps)
       apply(rule transpile_rules IH)+
       done
   qed
 qed
 
-
-
-  
-
-
-thm refines_HT'[OF _ refines_binarysearch]
-
-
 lemma flatten_correct: "sorted xs \<Longrightarrow> r \<le> length xs \<Longrightarrow> l \<le> r \<Longrightarrow>
-   <a \<mapsto>\<^sub>a xs > aahh l r x a
+   <a \<mapsto>\<^sub>a xs > binarysearch_flat l r x a
        <\<lambda>ra. a \<mapsto>\<^sub>a xs * \<up> (ra = (\<exists>i\<ge>l. i < r \<and> xs ! i = x))>\<^sub>t"
   apply(rule refines_HT) 
      apply(rule refines_binarysearch)
@@ -100,15 +90,15 @@ qed
 
 definition comb :: "nat \<Rightarrow> (nat \<Rightarrow> nat \<Rightarrow>  'a Heap_Time_Monad.Heap) \<Rightarrow> (nat \<Rightarrow>  'b Heap_Time_Monad.Heap) \<Rightarrow> ('a*'b) Heap_Time_Monad.Heap"
     where "comb n f g = do { fx \<leftarrow> f n n; gx \<leftarrow> g n; Heap_Time_Monad.return (fx,gx) } "
-term Pure.imp
-term "refines v t"
+
+
 transpile_define comb': comb_def
-print_theorems
 transpile_prove comb' comb
-print_theorems
  
-transpile_define imp_for'2: imp_for'.simps 
- 
+(* transpile_define TEST: imp_for'.simps 
+ would emit Error: "Recursive higher-order functions are not supported!"
+*)
+
 section "Example -- MergeSort"
 
 
@@ -127,9 +117,6 @@ transpile_prove mergeinto' mergeinto
 
 transpile_define merge_sort_impl': merge_sort_impl.simps
 transpile_prove merge_sort_impl' merge_sort_impl
-print_theorems
-
-thm prod.case
 
 lemma merge_sort_impl'_correct:
   "<p \<mapsto>\<^sub>a xs> merge_sort_impl' p <\<lambda>_. p \<mapsto>\<^sub>a sort xs>\<^sub>t" 
@@ -140,14 +127,11 @@ lemma merge_sort_impl'_correct:
   apply (simp add: forget_it)
   done
 
-
 section \<open>Example -- Dynamic Array\<close>
 
 lemma [transpile_rules]: "(\<And>al ar. refines (f' al ar) (f al ar)) \<Longrightarrow>
     refines (case x  of  Dyn_Array al ar \<Rightarrow> f' al ar) (case x  of  Dyn_Array al ar \<Rightarrow> f al ar)" 
   by(auto split: dynamic_array.splits)
-
-
 
 transpile_define array_copy': array_copy.simps
 transpile_replay array_copy' array_copy
@@ -179,7 +163,6 @@ transpile_prove dyn_array_new' dyn_array_new
 
 transpile_define dfilter_impl': dfilter_impl_def
 transpile_prove dfilter_impl' dfilter_impl
-print_theorems
 
 lemma "<a \<mapsto>\<^sub>a xs> dfilter_impl' a P
        <\<lambda>r. a \<mapsto>\<^sub>a xs * forget (dyn_array (filter P xs) r)>\<^sub>t"
@@ -192,14 +175,13 @@ lemma "<a \<mapsto>\<^sub>a xs> dfilter_impl' a P
 
 export_code dfilter_impl' in SML
 
-
 transpile_define destroy': destroy_def
 transpile_prove destroy' destroy
 
 
 subsection \<open>Example -- binarysearch\<close>
 
-transpile_define   binarysearch': binarysearch.simps
+transpile_define binarysearch': binarysearch.simps
 transpile_prove binarysearch' binarysearch
 
 lemma binarysearch'_HT: "sorted xs \<Longrightarrow> r \<le> length xs \<Longrightarrow> l \<le> r \<Longrightarrow>
@@ -210,7 +192,6 @@ lemma binarysearch'_HT: "sorted xs \<Longrightarrow> r \<le> length xs \<Longrig
     apply(rule binarysearch_correct')
       apply (simp_all  add: forget_it) 
   done
-
 
 section "Example -- Red Black Tree"
 
@@ -231,7 +212,6 @@ schematic_goal forget_rbt_map_assn: "forget (rbt_map_assn M b) = ?G"
   by(rule refl)
 concrete_definition rbt_map_assn_flat uses forget_rbt_map_assn
 lemmas [forget_it] = rbt_map_assn_flat.refine
-thm rbt_map_assn_flat_def
 
 transpile_define get_color': get_color_def
 transpile_prove get_color' get_color
@@ -249,8 +229,7 @@ transpile_define btree_balanceR': btree_balanceR_def
 transpile_prove btree_balanceR' btree_balanceR 
 
 transpile_define btree_balance': btree_balance_def
-transpile_prove btree_balance' btree_balance
- 
+transpile_prove btree_balance' btree_balance 
 
 transpile_define btree_constr': btree_constr_def
 transpile_prove btree_constr' btree_constr 
@@ -317,7 +296,7 @@ lemma rbt_delete'_HT:  "<rbt_map_assn_flat M b>
 transpile_define rbt_empty': RBTree_Impl.tree_empty_def
 transpile_prove rbt_empty' RBTree_Impl.tree_empty 
  
-theorem rbt_empty'_rule:
+theorem rbt_empty'_rule:       
   "<emp> rbt_empty' <rbt_map_assn_flat empty_map>"
   apply(rule refines_HT) 
      apply(rule Transpile_Tests.rbt_empty'.correct_translate)
@@ -353,7 +332,6 @@ schematic_goal forget_skew_heap_mset: "forget (skew_heap_mset T b) = ?G"
   apply (subst forget_it forget_btree)+
   by (rule refl)
 concrete_definition skew_heap_mset_flat uses forget_skew_heap_mset
-print_theorems
 lemmas [forget_it] =  skew_heap_mset_flat.refine 
 
 transpile_define skew_heap_merge_impl': merge_impl.simps
@@ -372,7 +350,6 @@ lemma skew_heap_merge'_rule:
 
 transpile_define skew_heap_constr': skew_heap_constr_def[unfolded tree_constr_def]
 transpile_prove skew_heap_constr' skew_heap_constr 
-
 
 transpile_define skew_heap_insert_impl': insert_impl_def
 transpile_prove skew_heap_insert_impl'  insert_impl  
@@ -403,10 +380,6 @@ lemma skew_heap_del_min_rule'_rule:
   apply (simp add: forget_it) 
   done
 
-term skew_heap_empty
-thm skew_heap_empty_rule''
-
-
 transpile_define skew_heap_empty': skew_heap_empty_def[unfolded Tree_Impl.tree_empty_def]
 transpile_prove skew_heap_empty' skew_heap_empty  
 
@@ -421,275 +394,7 @@ lemma "<emp> skew_heap_empty' <skew_heap_mset_flat {#}>\<^sub>t"
 export_code skew_heap_empty' skew_heap_insert_impl'
           skew_heap_del_min_impl' skew_heap_insert_impl' in SML
 
-section "Examples -- with fixp combinator"
 
 
-subsection \<open>Remove Duplicates\<close>
-
-lemma [transpile_rules]:   "refines (return v) (ureturn v)"
-  unfolding refines_def return_def ureturn_def
-    Heap_Time_Monad.effect_def Heap_Monad.effect_def
-    Heap_Time_Monad.heap_def Heap_Monad.heap_def
-  by auto
-
-lemma [transpile_rules]:   "
-  (\<And>a b. refines (f' a b) (f a b)) \<Longrightarrow>
-  refines (case x of (a,b) \<Rightarrow> f' a b) (case x of (a,b) \<Rightarrow> f a b)"
-  by (auto split: prod.splits)
-
-transpile_define set_empty': set_empty_def
-transpile_prove set_empty' set_empty
-
-transpile_define rbt_mem': rbt_mem_def
-transpile_prove rbt_mem' rbt_mem
-
-transpile_define rbt_set_insert': rbt_set_insert_def
-transpile_prove rbt_set_insert' rbt_set_insert
-
-transpile_define remdups_impl': remdups_impl_def[unfolded heap_WHILET_def, THEN meta_eq_to_obj_eq]
-transpile_prove  remdups_impl' remdups_impl
-print_theorems
-
-lemmas [code del] = remdups_impl'_def
-thm remdups_impl'_def[unfolded to_meta_eq, unfolded   ]
-prepare_code_thms remdups_impl'_def[unfolded to_meta_eq, unfolded   ]
- 
-definition remdups_impl'_nat :: "nat list \<Rightarrow> nat dynamic_array Heap_Monad.Heap" where
-  "remdups_impl'_nat as \<equiv>remdups_impl' as"                 
-prepare_code_thms remdups_impl'_nat_def[unfolded remdups_impl'_def]
- 
-export_code remdups_impl'_nat in SML module_name REMDUPS
-
-
-subsection \<open>Kruskal\<close>
-
-
-term kruskal'
-thm kruskal'_def
-
-term kruskal_final
-thm kruskal_final_def
-
-thm Kruskal_Time.Kruskal_final.E
-
-term Kruskal_intermediate_Impl.kruskal
-
-
-lemma list_case_reines[transpile_rules]:
-    "refines f' f 
-    \<Longrightarrow> (\<And>x xs. refines (g' x xs) (g x xs))
-    \<Longrightarrow>  refines (case x of [] \<Rightarrow> f' | (x#xs) \<Rightarrow> g' x xs)
-         (case x of [] \<Rightarrow> f | (x#xs) \<Rightarrow> g x xs)"
-  by (auto split: list.splits)
-
-
-
-lemma case_wrap_refine[transpile_rules]:
-  "(\<And>a. refines (f' a) (f a)) \<Longrightarrow> refines (case_wrap f' x) (case_wrap f x)"
-  by(auto split: wrap.splits)
-
-transpile_define maxn'': maxn'.simps
-transpile_replay maxn'' maxn'
-transpile_prove maxn'' maxn'
-
-transpile_define maxn': maxn_def
-transpile_prove maxn' maxn
-
-transpile_define sortEdges'': sortEdges'_def
-transpile_prove sortEdges'' sortEdges'
-
-thm uf_init_def
-transpile_define uf_init': uf_init_def[THEN meta_eq_to_obj_eq]
-transpile_prove uf_init' uf_init
-
-transpile_define uf_rep_of': uf_rep_of.simps
-transpile_prove uf_rep_of' uf_rep_of 
-
-transpile_define uf_compress': uf_compress.simps
-transpile_prove uf_compress' uf_compress 
-
-transpile_define uf_rep_of_c': uf_rep_of_c_def[THEN meta_eq_to_obj_eq]
-transpile_prove uf_rep_of_c' uf_rep_of_c
-
-transpile_define uf_cmp': uf_cmp_def[THEN meta_eq_to_obj_eq]
-transpile_prove uf_cmp' uf_cmp
-
-transpile_define uf_union' : uf_union_def[THEN meta_eq_to_obj_eq]
-transpile_prove uf_union' uf_union
- 
-thm  kruskal_final_def[of getEdges_impl]
-definition "kruskal_final_final as = kruskal_final (Heap_Time_Monad.return as)"
-thm kruskal_final_final_def[unfolded kruskal_final_def kruskal'_def]
-transpile_define kruskal_final': kruskal_final_final_def[unfolded kruskal_final_def kruskal'_def]
-transpile_prove kruskal_final' kruskal_final
-
-thm kruskal_final'_def
-definition "Kruskal_fun as \<equiv> do { k \<leftarrow> kruskal_final' as; a \<leftarrow> destroy' k; Array.freeze a}"
-prepare_code_thms (in -) Kruskal_fun_def[unfolded kruskal_final'_def]
-print_theorems
- 
-export_code integer_of_int int_of_integer
-    integer_of_nat  nat_of_integer
-    Kruskal_fun in SML module_name KRUSKAL
- 
-subsection \<open>Floyd-Warshall\<close>
-
-
-lemma "(\<And>x. f x = g x) \<Longrightarrow> f = g" apply (rule ext) by simp
-lemma kl: "f = g \<Longrightarrow> (\<And>x. f x = g x)"  
-  by auto
-
-transpile_define mtx_get': mtx_get_def
-transpile_prove mtx_get' mtx_get
-
-transpile_define mtx_set': mtx_set_def
-transpile_prove mtx_set' mtx_set
-
-term fw_upd_impl
-thm fw_upd_impl_def
-transpile_define fw_upd_impl': fw_upd_impl_def[THEN meta_eq_to_obj_eq, 
-    THEN kl, THEN kl, THEN kl, THEN kl, unfolded PR_CONST_def]
-transpile_prove fw_upd_impl' fw_upd_impl
-
-
-term fw_impl
-thm fw_impl_def
-thm fw_impl_def[THEN meta_eq_to_obj_eq]
-transpile_define fw_impl': fw_impl_def[THEN meta_eq_to_obj_eq, THEN kl ]
-transpile_prove fw_impl' fw_impl
-lemmas [code del] = fw_impl'_def
-thm fw_impl'_def
-prepare_code_thms fw_impl'_def[unfolded to_meta_eq] 
-print_theorems
-
-subsection "Edmonds Karp"
-
-
-
-thm Network_Impl.edka_imp_correct
-term edka_imp
-
-thm refines_imp_for
-
-transpile_define mtx_tabulate': mtx_tabulate_def[THEN meta_eq_to_obj_eq]
-transpile_prove mtx_tabulate' mtx_tabulate
-
-transpile_define init_cf_impl': init_cf_impl_def[THEN meta_eq_to_obj_eq]
-transpile_prove init_cf_impl' init_cf_impl
-
-transpile_define edka_imp_tabulate': edka_imp_tabulate_def[THEN meta_eq_to_obj_eq]
-transpile_prove edka_imp_tabulate' edka_imp_tabulate
-
-transpile_define new_liam': new_liam_def
-transpile_prove new_liam' new_liam
-
-transpile_define update_liam': update_liam_def
-transpile_prove update_liam' new_liam
-
-transpile_define nth_liam': nth_liam_def
-transpile_prove nth_liam' nth_liam
-
-transpile_define dom_member_liam': dom_member_liam_def
-transpile_prove dom_member_liam' dom_member_liam
-
-transpile_define os_empty': os_empty_def
-transpile_prove os_empty' os_empty
-
-transpile_define os_prepend': os_prepend_def
-transpile_prove os_prepend' os_prepend
-
-transpile_define os_pop': os_pop_def
-transpile_prove os_pop' os_pop
-
-transpile_define list_set_pick_extract': list_set_pick_extract_def[ THEN kl ]
-transpile_prove list_set_pick_extract' list_set_pick_extract
-
-transpile_define list_set_empty': list_set_empty_def
-transpile_prove list_set_empty' list_set_empty
-
-transpile_define list_set_insert': list_set_insert_def
-transpile_prove list_set_insert' list_set_insert
-
-transpile_define list_set_isempty': list_set_isempty_def[unfolded os_is_empty_def, THEN kl ]
-transpile_prove list_set_isempty' list_set_isempty
-
-transpile_define init_state_impl': init_state_impl_def[THEN meta_eq_to_obj_eq]
-transpile_prove init_state_impl' init_state_impl
-
-transpile_define oappend': oappend_def
-transpile_prove oappend' oappend
-
- 
-transpile_define bfs_impl': bfs_impl_def[THEN meta_eq_to_obj_eq]
-thm bfs_impl'_def
-print_theorems
-transpile_prove bfs_impl' bfs_impl
-print_theorems
-lemmas [code del] = bfs_impl'_def
-prepare_code_thms bfs_impl'_def[unfolded to_meta_eq] 
-
-transpile_define ps_get_imp': ps_get_imp_def[THEN meta_eq_to_obj_eq]
-transpile_prove ps_get_imp' ps_get_imp
-thm succ_imp_def
-transpile_define succ_imp': succ_imp_def[THEN meta_eq_to_obj_eq, unfolded PR_CONST_def]
-transpile_prove succ_imp' succ_imp
-lemmas [code del] = succ_imp'_def
-prepare_code_thms succ_imp'_def[unfolded to_meta_eq] 
-thm succ_imp'_def
- 
-transpile_define bfsi'': bfsi'_def[THEN meta_eq_to_obj_eq, unfolded split_beta']
-transpile_prove bfsi'' bfsi'
-thm bfsi''_def
-
-transpile_define resCap_imp': resCap_imp_def[THEN meta_eq_to_obj_eq, unfolded PR_CONST_def]
-transpile_prove resCap_imp' resCap_imp
-lemmas [code del] = resCap_imp'_def
-prepare_code_thms resCap_imp'_def[unfolded to_meta_eq] 
-
-transpile_define augment_imp': augment_imp_def[THEN meta_eq_to_obj_eq, THEN kl,THEN kl,THEN kl,unfolded PR_CONST_def]
-transpile_prove augment_imp' augment_imp
-lemmas [code del] = augment_imp'_def
-prepare_code_thms augment_imp'_def[unfolded to_meta_eq] 
-
-
-transpile_define edka_imp_run': edka_imp_run_def[THEN meta_eq_to_obj_eq]
-transpile_prove edka_imp_run' edka_imp_run
-lemmas [code del] = edka_imp_run'_def
-prepare_code_thms edka_imp_run'_def[unfolded to_meta_eq] 
-
-transpile_define edka_imp': edka_imp_def[THEN meta_eq_to_obj_eq]
-transpile_prove edka_imp' edka_imp
-thm edka_imp'_def
-
-lemmas [code] = imp_for''.simps
-
-definition "edka c s t N am = do {
-          res \<leftarrow> edka_imp c s t N am;
-          r \<leftarrow> Array_Time.freeze res;
-          Heap_Time_Monad.return (r, length r)}"
-
-transpile_define  edka': edka_def
-transpile_prove  edka' edka
- 
-
-export_code integer_of_int int_of_integer
-    integer_of_nat  nat_of_integer
- edka' in SML module_name EDKA
-
-section "partial_function strangeness"
-
-thm rbt_ins.raw_induct (* no tuple *)
-thm btree_combine.raw_induct (* no tuple *)
-thm binarysearch.raw_induct (* tuple *)
-thm rbt_search.raw_induct (* tuple *)
-thm rbt_del.raw_induct (* tuple *)
-
-partial_function (heap_time) rbt_del2 ::
-  "'a::{heap,linorder} \<Rightarrow> ('a, 'b::heap) btree \<Rightarrow> ('a, 'b) btree Heap_Time_Monad.Heap" where
-  "rbt_del2 x p = (case p of
-     None \<Rightarrow> Heap_Time_Monad.return None
-   | Some pp \<Rightarrow> do {
-      t \<leftarrow> !pp;rbt_del2 x (RBTree_Impl.lsub t)})"
-thm rbt_del2.raw_induct (* tuple *)
 
 end
