SepLogicTime/Transpile_Tests_Sepref.thy
@@ -1,0 +1,238 @@
+theory Transpile_Tests_Sepref
+imports 
+  Transpile_Tests
+ "SeprefTime.Remdups" "SeprefTime.Kruskal_Time" 
+ "SeprefTime.FW_Code" "SeprefTime.EdmondsKarp_Time"
+ "HOL-Library.Code_Target_Numeral"
+begin
+
+section "Examples -- with fixp combinator"
+
+subsection \<open>Remove Duplicates\<close>
+
+lemma [transpile_rules]:   "refines (return v) (ureturn v)"
+  unfolding refines_def return_def ureturn_def
+    Heap_Time_Monad.effect_def Heap_Monad.effect_def
+    Heap_Time_Monad.heap_def Heap_Monad.heap_def
+  by auto
+
+transpile_define set_empty': set_empty_def
+transpile_prove set_empty' set_empty
+
+transpile_define rbt_mem': rbt_mem_def
+transpile_prove rbt_mem' rbt_mem
+
+transpile_define rbt_set_insert': rbt_set_insert_def
+transpile_prove rbt_set_insert' rbt_set_insert
+
+transpile_define remdups_impl': remdups_impl_def[unfolded heap_WHILET_def, THEN meta_eq_to_obj_eq]
+transpile_prove  remdups_impl' remdups_impl
+print_theorems
+
+lemmas [code del] = remdups_impl'_def
+thm remdups_impl'_def[unfolded to_meta_eq, unfolded   ]
+prepare_code_thms remdups_impl'_def[unfolded to_meta_eq, unfolded   ]
+ 
+definition remdups_impl'_nat :: "nat list \<Rightarrow> nat dynamic_array Heap_Monad.Heap" where
+  "remdups_impl'_nat as \<equiv>remdups_impl' as"                 
+prepare_code_thms remdups_impl'_nat_def[unfolded remdups_impl'_def]
+ 
+export_code remdups_impl'_nat in SML module_name REMDUPS
+
+subsection \<open>Kruskal\<close>
+
+lemma list_case_refines[transpile_rules]:
+    "refines f' f 
+    \<Longrightarrow> (\<And>x xs. refines (g' x xs) (g x xs))
+    \<Longrightarrow>  refines (case x of [] \<Rightarrow> f' | (x#xs) \<Rightarrow> g' x xs)
+         (case x of [] \<Rightarrow> f | (x#xs) \<Rightarrow> g x xs)"
+  by (auto split: list.splits)
+
+lemma case_wrap_refine[transpile_rules]:
+  "(\<And>a. refines (f' a) (f a)) \<Longrightarrow> refines (case_wrap f' x) (case_wrap f x)"
+  by(auto split: wrap.splits)
+
+transpile_define maxn'': maxn'.simps
+transpile_replay maxn'' maxn'
+transpile_prove maxn'' maxn'
+
+transpile_define maxn': maxn_def
+transpile_prove maxn' maxn
+
+transpile_define sortEdges'': sortEdges'_def
+transpile_prove sortEdges'' sortEdges'
+
+transpile_define uf_init': uf_init_def[THEN meta_eq_to_obj_eq]
+transpile_prove uf_init' uf_init
+
+transpile_define uf_rep_of': uf_rep_of.simps
+transpile_prove uf_rep_of' uf_rep_of 
+
+transpile_define uf_compress': uf_compress.simps
+transpile_prove uf_compress' uf_compress 
+
+transpile_define uf_rep_of_c': uf_rep_of_c_def[THEN meta_eq_to_obj_eq]
+transpile_prove uf_rep_of_c' uf_rep_of_c
+
+transpile_define uf_cmp': uf_cmp_def[THEN meta_eq_to_obj_eq]
+transpile_prove uf_cmp' uf_cmp
+
+transpile_define uf_union' : uf_union_def[THEN meta_eq_to_obj_eq]
+transpile_prove uf_union' uf_union
+ 
+thm  kruskal_final_def[of getEdges_impl]
+definition "kruskal_final_final as = kruskal_final (Heap_Time_Monad.return as)"
+thm kruskal_final_final_def[unfolded kruskal_final_def kruskal'_def]
+transpile_define kruskal_final': kruskal_final_final_def[unfolded kruskal_final_def kruskal'_def]
+transpile_prove kruskal_final' kruskal_final
+
+thm kruskal_final'_def
+definition "Kruskal_fun as \<equiv> do { k \<leftarrow> kruskal_final' as; a \<leftarrow> destroy' k; Array.freeze a}"
+prepare_code_thms (in -) Kruskal_fun_def[unfolded kruskal_final'_def]
+print_theorems
+ 
+export_code integer_of_int int_of_integer
+    integer_of_nat  nat_of_integer
+    Kruskal_fun in SML module_name KRUSKAL
+ 
+subsection \<open>Floyd-Warshall\<close>
+
+
+lemma "(\<And>x. f x = g x) \<Longrightarrow> f = g" apply (rule ext) by simp
+lemma kl: "f = g \<Longrightarrow> (\<And>x. f x = g x)"  
+  by auto
+
+transpile_define mtx_get': mtx_get_def
+transpile_prove mtx_get' mtx_get
+
+transpile_define mtx_set': mtx_set_def
+transpile_prove mtx_set' mtx_set
+
+transpile_define fw_upd_impl': fw_upd_impl_def[THEN meta_eq_to_obj_eq, 
+    THEN kl, THEN kl, THEN kl, THEN kl, unfolded PR_CONST_def]
+transpile_prove fw_upd_impl' fw_upd_impl
+
+transpile_define fw_impl': fw_impl_def[THEN meta_eq_to_obj_eq, THEN kl ]
+transpile_prove fw_impl' fw_impl
+lemmas [code del] = fw_impl'_def
+
+prepare_code_thms fw_impl'_def[unfolded to_meta_eq] 
+
+
+subsection "Edmonds Karp"
+
+transpile_define mtx_tabulate': mtx_tabulate_def[THEN meta_eq_to_obj_eq]
+transpile_prove mtx_tabulate' mtx_tabulate
+
+transpile_define init_cf_impl': init_cf_impl_def[THEN meta_eq_to_obj_eq]
+transpile_prove init_cf_impl' init_cf_impl
+
+transpile_define edka_imp_tabulate': edka_imp_tabulate_def[THEN meta_eq_to_obj_eq]
+transpile_prove edka_imp_tabulate' edka_imp_tabulate
+
+transpile_define new_liam': new_liam_def
+transpile_prove new_liam' new_liam
+
+transpile_define update_liam': update_liam_def
+transpile_prove update_liam' new_liam
+
+transpile_define nth_liam': nth_liam_def
+transpile_prove nth_liam' nth_liam
+
+transpile_define dom_member_liam': dom_member_liam_def
+transpile_prove dom_member_liam' dom_member_liam
+
+transpile_define os_empty': os_empty_def
+transpile_prove os_empty' os_empty
+
+transpile_define os_prepend': os_prepend_def
+transpile_prove os_prepend' os_prepend
+
+transpile_define os_pop': os_pop_def
+transpile_prove os_pop' os_pop
+
+transpile_define list_set_pick_extract': list_set_pick_extract_def[ THEN kl ]
+transpile_prove list_set_pick_extract' list_set_pick_extract
+
+transpile_define list_set_empty': list_set_empty_def
+transpile_prove list_set_empty' list_set_empty
+
+transpile_define list_set_insert': list_set_insert_def
+transpile_prove list_set_insert' list_set_insert
+
+transpile_define list_set_isempty': list_set_isempty_def[unfolded os_is_empty_def, THEN kl ]
+transpile_prove list_set_isempty' list_set_isempty
+
+transpile_define init_state_impl': init_state_impl_def[THEN meta_eq_to_obj_eq]
+transpile_prove init_state_impl' init_state_impl
+
+transpile_define oappend': oappend_def
+transpile_prove oappend' oappend
+ 
+transpile_define bfs_impl': bfs_impl_def[THEN meta_eq_to_obj_eq]
+transpile_prove bfs_impl' bfs_impl
+lemmas [code del] = bfs_impl'_def
+prepare_code_thms bfs_impl'_def[unfolded to_meta_eq] 
+
+transpile_define ps_get_imp': ps_get_imp_def[THEN meta_eq_to_obj_eq]
+transpile_prove ps_get_imp' ps_get_imp
+
+transpile_define succ_imp': succ_imp_def[THEN meta_eq_to_obj_eq, unfolded PR_CONST_def]
+transpile_prove succ_imp' succ_imp
+lemmas [code del] = succ_imp'_def
+prepare_code_thms succ_imp'_def[unfolded to_meta_eq] 
+ 
+transpile_define bfsi'': bfsi'_def[THEN meta_eq_to_obj_eq, unfolded split_beta']
+transpile_prove bfsi'' bfsi'
+
+transpile_define resCap_imp': resCap_imp_def[THEN meta_eq_to_obj_eq, unfolded PR_CONST_def]
+transpile_prove resCap_imp' resCap_imp
+lemmas [code del] = resCap_imp'_def
+prepare_code_thms resCap_imp'_def[unfolded to_meta_eq] 
+
+transpile_define augment_imp': augment_imp_def[THEN meta_eq_to_obj_eq, THEN kl,THEN kl,THEN kl,unfolded PR_CONST_def]
+transpile_prove augment_imp' augment_imp
+lemmas [code del] = augment_imp'_def
+prepare_code_thms augment_imp'_def[unfolded to_meta_eq] 
+
+transpile_define edka_imp_run': edka_imp_run_def[THEN meta_eq_to_obj_eq]
+transpile_prove edka_imp_run' edka_imp_run
+lemmas [code del] = edka_imp_run'_def
+prepare_code_thms edka_imp_run'_def[unfolded to_meta_eq] 
+
+transpile_define edka_imp': edka_imp_def[THEN meta_eq_to_obj_eq]
+transpile_prove edka_imp' edka_imp
+
+lemmas [code] = imp_for''.simps
+
+definition "edka c s t N am = do {
+          res \<leftarrow> edka_imp c s t N am;
+          r \<leftarrow> Array_Time.freeze res;
+          Heap_Time_Monad.return (r, length r)}"
+
+transpile_define  edka': edka_def
+transpile_prove  edka' edka
+ 
+
+export_code integer_of_int int_of_integer
+    integer_of_nat  nat_of_integer
+ edka' in SML module_name EDKA
+
+section "partial_function strangeness"
+
+thm rbt_ins.raw_induct (* no tuple *)
+thm btree_combine.raw_induct (* no tuple *)
+thm binarysearch.raw_induct (* tuple *)
+thm rbt_search.raw_induct (* tuple *)
+thm rbt_del.raw_induct (* tuple *)
+
+partial_function (heap_time) rbt_del2 ::
+  "'a::{heap,linorder} \<Rightarrow> ('a, 'b::heap) btree \<Rightarrow> ('a, 'b) btree Heap_Time_Monad.Heap" where
+  "rbt_del2 x p = (case p of
+     None \<Rightarrow> Heap_Time_Monad.return None
+   | Some pp \<Rightarrow> do {
+      t \<leftarrow> !pp;rbt_del2 x (RBTree_Impl.lsub t)})"
+thm rbt_del2.raw_induct (* tuple *)
+
+
+end
